QuickSortInLean/AdjacentSorted.lean
@@ -1,0 +1,14 @@
+import QuickSortInLean.Order
+import QuickSortInLean.Vec
+
+theorem sorted_of_adjacentSorted {α : Type} [Order α] {n : Nat}
+  (arr : Vec α n)
+  (assms : ∀i : Nat, (isLt : i + 1 < n) → arr[i]'(Nat.lt_of_le_of_lt (Nat.le_succ ..) isLt) ≤o arr[i + 1]'isLt)
+  (j k : Nat) (kn : k < n) (jk : j ≤ k) :
+  arr[j]'(Nat.lt_of_le_of_lt jk kn) ≤o arr[k] := by
+  induction jk with
+  | refl => exact Order.refl
+  | step h ih =>
+    apply Order.trans
+    . exact ih (Nat.lt_of_le_of_lt (Nat.le_succ ..) kn)
+    . apply assms
