QuickSortInLean/QuickSortPermutation.lean
@@ -2,11 +2,11 @@ import QuickSortInLean.Permutation
 import QuickSortInLean.QuickSort
 import QuickSortInLean.Induction
 
-theorem partitionImpl_permuted {α : Type} [Ord α]
+def partitionImpl_permuted' {α : Type} [Ord α]
   {n : Nat} (arr : Vec α n) (first i j : Fin n)
   (fi : first ≤ i) (ij : i ≤ j) :
   permuted n first j arr (partitionImpl arr first i j fi ij).2 := by
-  induction arr, first, i, j, fi, ij using partitionImpl.induct with
+  induction arr, first, i, j, fi, ij using partitionImpl.induct' with
   | base arr first i j fi ij jn =>
     simp [*]
     exact .refl
@@ -17,32 +17,50 @@ theorem partitionImpl_permuted {α : Type} [Ord α]
     simp [*]
     apply permuted.step i j fi ij (Nat.le_refl _) (ih.cast_last (Nat.sub_le ..))
 
-theorem partition_permuted {α : Type} [Ord α]
+theorem partitionImpl_permuted {α : Type} [Ord α]
+  {n : Nat} (arr : Vec α n) (first i j : Fin n)
+  (fi : first ≤ i) (ij : i ≤ j) :
+  Nonempty (permuted n first j arr (partitionImpl arr first i j fi ij).2) := by
+  induction arr, first, i, j, fi, ij using partitionImpl.induct with
+  | case1 arr first i j fi ij lt jl h prev ih =>
+    unfold partitionImpl
+    simp [*]
+  | @case2 arr first i j fi ij lt jl h swapped mid hm arr' eq ih =>
+    unfold partitionImpl
+    simp [*] at *
+    have ⟨p₂⟩ := ih
+    have p₁ : permuted n first j arr swapped := .step i j fi ij (Nat.le_refl _) .refl
+    exact ⟨p₁.trans $ p₂.cast_last (Nat.sub_le ..)⟩
+  | case3 arr first i j fi ij jn =>
+    simp [partitionImpl, *]
+    exact ⟨.refl⟩
+
+def partition_permuted' {α : Type} [Ord α]
   {n : Nat} (arr : Vec α n) (first last : Fin n) (fl : first ≤ last) :
   permuted n first last arr (partition arr first last fl).2 := by
   let result := partition arr first last fl
   let mid := result.1
   simp [partition, dbgTraceIfShared]
-  let p := partitionImpl_permuted arr first last last fl (Nat.le_refl _)
+  let p := partitionImpl_permuted' arr first last last fl (Nat.le_refl _)
   exact permuted.trans p
     (.step first ⟨mid, Nat.lt_of_le_of_lt mid.property.2 last.isLt⟩ (Nat.le_refl _) mid.property.1 mid.property.2 .refl)
 
-theorem quickSortImpl_permuted {α : Type} [Ord α]
+def quickSortImpl_permuted {α : Type} [Ord α]
   {n : Nat} (arr : Vec α n) (first : Nat) (last : Fin n) :
   permuted n first last arr (quickSortImpl arr first last) := by
-  induction arr, first, last using quickSortImpl.induct with
+  induction arr, first, last using quickSortImpl.induct' with
   | base arr first last h =>
     simp [*]
     exact .refl
   | step arr first last lt parted eq ih₁ ih₂ =>
     simp [*]
-    let p := partition_permuted arr ⟨first, Nat.lt_trans lt last.isLt⟩ last (Nat.le_of_lt lt)
+    let p := partition_permuted' arr ⟨first, Nat.lt_trans lt last.isLt⟩ last (Nat.le_of_lt lt)
     rw [eq] at p
     exact permuted.trans
       (permuted.trans p (ih₁.cast_last (Nat.le_trans (Nat.sub_le ..) parted.1.property.2)))
       (ih₂.cast_first (Nat.le_trans parted.1.property.1 (Nat.le_succ _)))
 
-theorem quickSort'_permuted  {α : Type} [Ord α] {n : Nat} (arr : Vec α n) :
+def quickSort'_permuted  {α : Type} [Ord α] {n : Nat} (arr : Vec α n) :
   permuted n 0 (n - 1) arr (quickSort' arr) := by
   simp [quickSort']
   match Nat.decLt 0 n with
